Remove use of finite_image tycon in grammar theory.
This really was causing too much pain. The latest example of this was
the fact that I couldn’t pattern-match against token values because
mk_finite_image is not an officially recognised constructor.

examples/parsing/pegSampleScript.sml
@@ -4,20 +4,7 @@ open pegexecTheory
 
 val _ = new_theory "pegSample"
 
-
-val _ = overload_on("mkTok", ``mk_finite_image``)
-
-val _ = Hol_datatype`ftok = Plus | Times | Number | LParen | RParen`
-
-val _ = Hol_datatype`etok = EPlus | ETimes | ENumber of num | ELParen | ERParen`
-
-val categorise_def = Define`
-  categorise EPlus = mkTok Plus ∧
-  categorise ETimes = mkTok Times ∧
-  categorise (ENumber n) = mkTok Number ∧
-  categorise ELParen = mkTok LParen ∧
-  categorise ERParen = mkTok RParen
-`;
+val _ = Hol_datatype`tok = Plus | Times | Number of num | LParen | RParen`
 
 local open stringTheory in end
 
@@ -27,18 +14,15 @@ val _ = Hol_datatype `
        | XTimes of expr => expr
        | XList of expr list`;
 
-val _ = overload_on("mkTok", ``mk_finite_image``)
-
-
-val ty = ty_antiq ``:(ftok, string, expr, etok) pegsym``
-val lift_enumber_def = Define`
-  lift_enumber (ENumber n) = XN n
+val ty = ty_antiq ``:(tok, string, expr) pegsym``
+val lift_number_def = Define`
+  lift_number (Number n) = XN n
 `;
 
-val nrule = ``tok (mkTok Number) lift_enumber : ^ty``
+val nrule = ``tok (λt. case t of Number n => T | _ => F) lift_number : ^ty``
 val paren_rule =
-  ``seq (tok (mkTok LParen) (K (XN 0)))
-        (seq (nt (INL "expr") I) (tok (mkTok RParen) (K (XN 0))) K)
+  ``seq (tok ((=) LParen) (K (XN 0)))
+        (seq (nt (INL "expr") I) (tok ((=) RParen) (K (XN 0))) K)
         (K I) : ^ty``
 
 val termpair =
@@ -52,7 +36,7 @@ val leftassoc_def = Define`
 
 val factorpair = ``(INL "factor" : string inf,
                     seq (rpt (seq (nt (INL "term") I)
-                                  (tok (mkTok Times) (K ARB))
+                                  (tok ((=) Times) (K ARB))
                                   K)
                              XList)
                         (nt (INL "term") I)
@@ -60,7 +44,7 @@ val factorpair = ``(INL "factor" : string inf,
 
 val exprpair = ``(INL "expr" : string inf,
                   seq (rpt (seq (nt (INL "factor") I)
-                                (tok (mkTok Plus) (K ARB))
+                                (tok ((=) Plus) (K ARB))
                                 K)
                            XList)
                       (nt (INL "factor") I)
@@ -68,33 +52,14 @@ val exprpair = ``(INL "expr" : string inf,
 
 val rules = ``FEMPTY |+ ^exprpair |+ ^factorpair |+ ^termpair``
 
-val G = ``<| start := nt (INL "expr") I; rules := ^rules; cf := categorise |>``
+val G = ``<| start := nt (INL "expr") I; rules := ^rules |>``
 
-val testexp = ``[ENumber 3; EPlus; ENumber 4; ETimes; ENumber 5]``
+val testexp = ``[Number 3; Plus; Number 4; Times; Number 5]``
 
 open lcsymtacs
-val mkTok_inverse =
-    fcpTheory.finite_image_tybij |> CONJUNCT2 |> SPEC_ALL |> EQ_IMP_RULE |> #1
-                                 |> BETA_RULE
-                                 |> REWRITE_RULE [ASSUME ``FINITE univ(:'a)``]
-                                 |> DISCH_ALL
-
-val univ_ftok = store_thm(
-  "univ_ftok",
-  ``univ(:ftok) = {LParen; RParen; Number; Plus; Times}``,
-  simp[pred_setTheory.EXTENSION] >> Cases >> simp[]);
-
-val mkTok_11 = store_thm(
-  "mkTok_11",
-  ``mkTok (x:ftok) = mkTok (y:ftok) ⇔ x = y``,
-  simp[EQ_IMP_THM] >>
-  disch_then (MP_TAC o AP_TERM ``dest_finite_image : ftok tok -> ftok``) >>
-  simp[univ_ftok, mkTok_inverse]);
-
 val _ = let
   open computeLib
 in
-  add_persistent_funs ["mkTok_11"];
   set_skip the_compset ``evalcase_CASE`` (SOME 1);
   set_skip the_compset ``option_CASE`` (SOME 1);
   set_skip the_compset ``COND`` (SOME 1)
@@ -105,15 +70,41 @@ end
 val result1 = save_thm(
   "result1",
   time EVAL ``peg_exec ^G (nt (INL "expr") I)
-                      [ENumber 1; EPlus; ENumber 2; ETimes; ENumber 4] []
+                      [Number 1; Plus; Number 2; Times; Number 4] []
                       done failed``)
 
 (* As of 5a18cdc17ff, takes 1.983s (ugh) *)
 val result2 = save_thm(
   "result2",
   time EVAL ``peg_exec ^G (nt (INL "expr") I)
-                      [ENumber 1; EPlus; ENumber 2; ETimes; ENumber 4;
-                       ETimes; ELParen; ENumber 3; EPlus; ENumber 1; ERParen]
+                      [Number 1; Plus; Number 2; Times; Number 4;
+                       Times; LParen; Number 3; Plus; Number 1; RParen]
+                      [] done failed``)
+
+val G_def = zDefine`G = <| start := nt (INL "expr") I; rules := ^rules |>`
+
+val Grules = store_thm(
+  "Grules",
+  ``G.rules ' (INL "expr") = ^(#2 (pairSyntax.dest_pair exprpair)) ∧
+    G.rules ' (INL "factor") = ^(#2 (pairSyntax.dest_pair factorpair)) ∧
+    G.rules ' (INL "term") = ^(#2 (pairSyntax.dest_pair termpair)) ∧
+    INL "expr" ∈ FDOM G.rules ∧
+    INL "term" ∈ FDOM G.rules ∧
+    INL "factor" ∈ FDOM G.rules``,
+  simp[G_def, finite_mapTheory.FAPPLY_FUPDATE_THM]);
+val _ = computeLib.add_persistent_funs ["Grules"]
+
+(* on a machine running PolyML 5.4.1, and where result2 takes 0.084s,
+   the following takes 0.028s
+
+   One further optimisation would be partially evaluate the actual
+   nt values against exec theorem and put the result into the compset
+*)
+val result2' = save_thm(
+  "result2'",
+  time EVAL ``peg_exec G (nt (INL "expr") I)
+                      [Number 1; Plus; Number 2; Times; Number 4;
+                       Times; LParen; Number 3; Plus; Number 1; RParen]
                       [] done failed``)
 
 
